src/Dafny/examples/fs/indirect_fs.dfy
@@ -197,12 +197,12 @@ module IndFs
       ensures ValidQ()
       ensures fresh(Repr)
       ensures data == imap pos: Pos {:trigger pos.idx.data?} | pos.idx.data? :: block0
-      ensures metadata == map ino: Ino {:trigger} :: Inode.Meta(0, Inode.InvalidType, Inode.Attrs.zero)
+      ensures metadata == map ino: Ino {:trigger} :: Inode.Meta.zero
     {
       this.fs := new Filesys.Init(d);
       this.to_blkno := imap pos: Pos {:trigger} :: 0 as Blkno;
       this.data := imap pos: Pos | pos.idx.data? :: block0;
-      this.metadata := map ino: Ino {:trigger} :: Inode.Meta(0, Inode.InvalidType, Inode.Attrs.zero);
+      this.metadata := map ino: Ino {:trigger} :: Inode.Meta.zero;
       new;
       assert ValidBasics() by { reveal fsValid(); }
       IndBlocks.to_blknos_zero();
